New jump instructions (#7)
Squashed commit of the following:

commit cc0a82404dc0883bd2b0bc7a350c696c776e9450
Author: June Rousseau <june.rousseau@cs.au.dk>
Date:   Tue Feb 11 12:16:21 2025 +0100

    Ignore malloc macros

commit 024d7e25e256e320c761a40a4765670bda6b359c
Author: June Rousseau <june.rousseau@cs.au.dk>
Date:   Tue Feb 11 12:14:04 2025 +0100

    Fix assert macros

commit bc7fd35b1c4be522523b647b1a454ab7adb59cdb
Author: June Rousseau <june.rousseau@cs.au.dk>
Date:   Tue Feb 11 11:16:13 2025 +0100

    Fix FTLR

commit e9eb7913f75610904e52bb24ac7a7d429e545656
Author: June Rousseau <june.rousseau@cs.au.dk>
Date:   Tue Feb 11 11:09:00 2025 +0100

    Proof FTLR Jnz

commit 45bf864574f2fdf4d64295c95ede9ccc3b0ae879
Author: June Rousseau <june.rousseau@cs.au.dk>
Date:   Tue Feb 11 11:04:24 2025 +0100

    Proof FTLR Jmp

commit e50e20a5199af89e288bf46f5408e13de9de1a21
Author: June Rousseau <june.rousseau@cs.au.dk>
Date:   Tue Feb 11 10:33:53 2025 +0100

    Proof FTLR Jalr

commit 2d7a6db7645ce9a357775d0eda25490503607151
Author: June Rousseau <june.rousseau@cs.au.dk>
Date:   Tue Feb 11 10:03:02 2025 +0100

    Fix WP rule Jalr: can fail

commit b629acae50d99db4888e1ed640b39a75eb0d426c
Author: June Rousseau <june.rousseau@cs.au.dk>
Date:   Tue Feb 11 09:36:42 2025 +0100

    Instanciated WP rules Jnz, and fixing proofmode

commit e113e43bbbfac0ff4ae7bf51287d7a88185ad519
Author: June Rousseau <june.rousseau@cs.au.dk>
Date:   Mon Feb 10 23:00:12 2025 +0100

    WP rules for Jmp, Jnz and Jalr

commit 79f13b22df0a233cd63185cdf6c2d41e3c5ae6fd
Author: June Rousseau <june.rousseau@cs.au.dk>
Date:   Mon Feb 10 22:32:22 2025 +0100

    Change opsem Jmp and Jnz to relative jump; and add instruction Jalr

theories/machine_base.v
@@ -175,8 +175,9 @@ Notation WCap p g b e a := (WSealable (SCap p g b e a)).
 Notation WSealRange p g b e a := (WSealable (SSealRange p g b e a)).
 
 Inductive instr: Type :=
-| Jmp (r: RegName)
-| Jnz (r1 r2: RegName)
+| Jmp (rimm: Z + RegName)
+| Jnz (rimm : Z + RegName) (rcond: RegName)
+| Jalr (rsrc: RegName)
 | Mov (dst: RegName) (src: Z + RegName)
 | Load (dst src: RegName)
 | Store (dst: RegName) (src: Z + RegName)
@@ -1588,8 +1589,8 @@ Proof.
 
   set (enc := fun e =>
       match e with
-      | Jmp r => GenNode 0 [GenLeaf (inl (inl r))]
-      | Jnz r1 r2 => GenNode 1 [GenLeaf (inl (inl r1)); GenLeaf (inl (inl r2))]
+      | Jmp r => GenNode 0 [GenLeaf (inr r)]
+      | Jnz r1 r2 => GenNode 1 [GenLeaf (inr r1); GenLeaf (inl (inl r2))]
       | Mov dst src => GenNode 2 [GenLeaf (inl (inl dst)); GenLeaf (inr src)]
       | Load dst src => GenNode 3 [GenLeaf (inl (inl dst)); GenLeaf (inl (inl src))]
       | Store dst src => GenNode 4 [GenLeaf (inl (inl dst)); GenLeaf (inr src)]
@@ -1619,11 +1620,12 @@ Proof.
       | LOr dst r1 r2 => GenNode 26 [GenLeaf (inl (inl dst)); GenLeaf (inr r1); GenLeaf (inr r2)]
       | LShiftL dst r1 r2 => GenNode 27 [GenLeaf (inl (inl dst)); GenLeaf (inr r1); GenLeaf (inr r2)]
       | LShiftR dst r1 r2 => GenNode 28 [GenLeaf (inl (inl dst)); GenLeaf (inr r1); GenLeaf (inr r2)]
+      | Jalr r => GenNode 29 [GenLeaf (inl (inl r))]
       end).
   set (dec := fun e =>
       match e with
-      | GenNode 0 [GenLeaf (inl (inl r))] => Jmp r
-      | GenNode 1 [GenLeaf (inl (inl r1)); GenLeaf (inl (inl r2))] => Jnz r1 r2
+      | GenNode 0 [GenLeaf (inr r) ] => Jmp r
+      | GenNode 1 [GenLeaf (inr r1); GenLeaf (inl (inl r2))] => Jnz r1 r2
       | GenNode 2 [GenLeaf (inl (inl dst)); GenLeaf (inr src)] => Mov dst src
       | GenNode 3 [GenLeaf (inl (inl dst)); GenLeaf (inl (inl src))] => Load dst src
       | GenNode 4 [GenLeaf (inl (inl dst)); GenLeaf (inr src)] => Store dst src
@@ -1653,6 +1655,7 @@ Proof.
       | GenNode 26 [GenLeaf (inl (inl dst)); GenLeaf (inr r1); GenLeaf (inr r2)] => LOr dst r1 r2
       | GenNode 27 [GenLeaf (inl (inl dst)); GenLeaf (inr r1); GenLeaf (inr r2)] => LShiftL dst r1 r2
       | GenNode 28 [GenLeaf (inl (inl dst)); GenLeaf (inr r1); GenLeaf (inr r2)] => LShiftR dst r1 r2
+      | GenNode 29 [GenLeaf (inl (inl r))] => Jalr r
       | _ => Fail (* dummy *)
       end).
   refine (inj_countable' enc dec _).
