theories/rules/rules_Jmp.v
@@ -17,61 +17,156 @@ Section cap_lang_rules.
   Implicit Types reg : gmap RegName Word.
   Implicit Types ms : gmap Addr Word.
 
-  Lemma wp_jmp_success E pc_p pc_g pc_b pc_e pc_a w r w' :
-    decodeInstrW w = Jmp r →
-     isCorrectPC (WCap pc_p pc_g pc_b pc_e pc_a) →
+  Inductive Jmp_failure (regs: Reg) (rimm: Z + RegName) :=
+  | Jmp_fail_no_imm:
+      z_of_argument regs rimm = None →
+      Jmp_failure regs rimm
+  | Jmp_fail_PC_overflow imm:
+      z_of_argument regs rimm = Some imm →
+      incrementPC_gen regs imm = None →
+      Jmp_failure regs rimm.
 
+  Inductive Jmp_spec (regs: Reg) (rimm: Z + RegName) : Reg → cap_lang.val → Prop :=
+  | Jmp_spec_success regs' imm :
+      z_of_argument regs rimm = Some imm →
+      incrementPC_gen regs imm = Some regs' →
+      Jmp_spec regs rimm regs' NextIV
+  | Jmp_spec_failure:
+      Jmp_failure regs rimm →
+      Jmp_spec regs rimm regs FailedV.
+
+  Lemma wp_Jmp Ep pc_p pc_g pc_b pc_e pc_a w rimm regs :
+    decodeInstrW w = Jmp rimm ->
+    isCorrectPC (WCap pc_p pc_g pc_b pc_e pc_a) →
+    regs !! PC = Some (WCap pc_p pc_g pc_b pc_e pc_a) →
+    regs_of (Jmp rimm) ⊆ dom regs →
+
+    {{{ ▷ pc_a ↦ₐ w ∗
+        ▷ [∗ map] k↦y ∈ regs, k ↦ᵣ y }}}
+      Instr Executable @ Ep
+    {{{ regs' retv, RET retv;
+        ⌜ Jmp_spec regs rimm regs' retv ⌝ ∗
+        pc_a ↦ₐ w ∗
+        [∗ map] k↦y ∈ regs', k ↦ᵣ y }}}.
+  Proof.
+    iIntros (Hinstr Hvpc HPC Dregs φ) "(>Hpc_a & >Hmap) Hφ".
+    iApply wp_lift_atomic_base_step_no_fork; auto.
+    iIntros (σ1 ns l1 l2 nt) "[ [Hr Hsr] Hm ] /=". destruct σ1 as [ [r sr] m]; cbn.
+    iDestruct (gen_heap_valid_inclSepM with "Hr Hmap") as %Hregs.
+    have ? := lookup_weaken _ _ _ _ HPC Hregs.
+    iDestruct (@gen_heap_valid with "Hm Hpc_a") as %Hpc_a; auto.
+    iModIntro. iSplitR. by iPureIntro; apply normal_always_base_reducible.
+    iNext. iIntros (e2 σ2 efs Hpstep).
+    apply prim_step_exec_inv in Hpstep as (-> & -> & (c & -> & Hstep)).
+    iIntros "_".
+    iSplitR; auto. eapply step_exec_inv in Hstep; eauto.
+    rewrite /exec /= in Hstep.
+
+    specialize (indom_regs_incl _ _ _ Dregs Hregs) as Hri.
+    unfold regs_of in Hri, Dregs.
+
+    destruct (z_of_argument regs rimm) as [imm|] eqn:Himm
+    ; pose proof Himm as H'imm
+    ; cycle 1.
+     { (* Failure: argument is not a constant (z_of_argument regs arg = None) *)
+       unfold z_of_argument in Himm, Hstep.
+       destruct rimm as [| rimm]; [ congruence |].
+       odestruct (Hri rimm) as [rimmv [Hrimm' Hrimm]].
+       { unfold regs_of_argument. set_solver+. }
+       rewrite Hrimm Hrimm' in Himm Hstep.
+       assert (c = Failed ∧ σ2 = (r, sr, m)) as (-> & ->).
+       { destruct_word rimmv; cbn in Hstep; try congruence; by simplify_pair_eq. }
+       iFailWP "Hφ" Jmp_fail_no_imm. }
+     apply (z_of_arg_mono _ r) in Himm; auto.
+     rewrite Himm in Hstep; simpl in Hstep.
+
+
+     destruct (incrementPC_gen regs imm) eqn:Hregs';
+       pose proof Hregs' as H'regs'; cycle 1.
+     {
+       assert (incrementPC_gen r imm = None) as HH.
+       { eapply incrementPC_gen_overflow_mono; first eapply Hregs' ; eauto. }
+       apply (incrementPC_gen_fail_updatePC_gen _ sr m) in HH. rewrite HH in Hstep.
+       assert (c = Failed ∧ σ2 = (r, sr, m)) as (-> & ->) by (inversion Hstep; auto).
+       iFailWP "Hφ" Jmp_fail_PC_overflow. }
+
+       eapply (incrementPC_gen_success_updatePC_gen _ sr m _ imm) in Hregs'
+         as (p'' & g'' & b' & e' & a'' & a''' & a_pc' & HPC'' & HuPC & ->).
+       eapply updatePC_gen_success_incl with (sregs':=sr) (m':=m) in HuPC; eauto.
+       rewrite HuPC in Hstep.
+       eassert ((c, σ2) = (NextI, _)) as HH.
+       { cbn in *; eauto. }
+       simplify_pair_eq.
+
+       iMod ((gen_heap_update_inSepM _ _ PC) with "Hr Hmap") as "[Hr Hmap]"; eauto.
+       iFrame.
+       iApply "Hφ". iFrame. iPureIntro. econstructor; eauto.
+  Qed.
+
+   Lemma wp_jmp_success_z Ep pc_p pc_g pc_b pc_e pc_a pc_a' w imm :
+     decodeInstrW w = Jmp (inl imm) →
+     isCorrectPC (WCap pc_p pc_g pc_b pc_e pc_a) →
+     (pc_a + imm)%a = Some pc_a' →
      {{{ ▷ PC ↦ᵣ WCap pc_p pc_g pc_b pc_e pc_a
          ∗ ▷ pc_a ↦ₐ w
-         ∗ ▷ r ↦ᵣ w' }}}
-       Instr Executable @ E
-       {{{ RET NextIV;
-           PC ↦ᵣ updatePcPerm w'
-           ∗ pc_a ↦ₐ w
-           ∗ r ↦ᵣ w' }}}.
-  Proof.
-    iIntros (Hinstr Hvpc ϕ) "(>HPC & >Hpc_a & >Hr) Hφ".
-    iApply wp_lift_atomic_base_step_no_fork; auto.
-    iIntros (σ1 ns l1 l2 nt) "[ [Hr0 Hsr] Hm ] /=". destruct σ1 as [ [r0 sr] m]; cbn.
-    iDestruct (@gen_heap_valid with "Hm Hpc_a") as %?; auto.
-    iDestruct (@gen_heap_valid with "Hr0 HPC") as %?.
-    iDestruct (@gen_heap_valid with "Hr0 Hr") as %Hr_r0.
-    iModIntro. iSplitR. by iPureIntro; apply normal_always_base_reducible.
-    iNext. iIntros (e2 σ2 efs Hpstep).
-    apply prim_step_exec_inv in Hpstep as (-> & -> & (c & -> & Hstep)).
-    iIntros "_".
-    iSplitR; auto. eapply step_exec_inv in Hstep; eauto.
-    unfold exec, exec_opt in Hstep. rewrite Hr_r0 /= in Hstep. simplify_pair_eq.
+     }}}
+       Instr Executable @ Ep
+     {{{ RET NextIV;
+         PC ↦ᵣ WCap pc_p pc_g pc_b pc_e pc_a'
+         ∗ pc_a ↦ₐ w
+     }}}.
+   Proof.
+     iIntros (Hinstr Hvpc Hpca' ϕ) "(>HPC & >Hpc_a) Hφ".
+     iDestruct (map_of_regs_1 with "HPC") as "Hmap".
+     iApply (wp_Jmp with "[$Hmap Hpc_a]"); eauto; simplify_map_eq; eauto.
+     { set_solver+. }
+     iNext. iIntros (regs' retv) "(#Hspec & Hpc_a & Hmap)".
+     iDestruct "Hspec" as %Hspec.
 
-    iMod (@gen_heap_update with "Hr0 HPC") as "[Hr0 HPC]". iFrame.
-    iApply "Hφ". by iFrame.
-  Qed.
+     destruct Hspec as [| * Hfail].
+     { (* Success *)
+       iApply "Hφ". iFrame.
+       incrementPC_inv as (?&?&?&?&?&?&?&?&?); simplify_map_eq.
+       rewrite insert_insert //.
+       iDestruct (regs_of_map_1 with "Hmap") as "(?&?)"; eauto; iFrame. }
+     { (* Failure (contradiction) *)
+       destruct Hfail; simplify_map_eq; eauto; try congruence.
+       incrementPC_inv as (?&?&?&?&?&?&?&?&?); simplify_map_eq; eauto ; congruence.
+     }
+   Qed.
 
-  Lemma wp_jmp_successPC E pc_p pc_g pc_b pc_e pc_a w :
-    decodeInstrW w = Jmp PC →
+   Lemma wp_jmp_success_reg Ep pc_p pc_g pc_b pc_e pc_a pc_a' w rimm imm:
+     decodeInstrW w = Jmp (inr rimm) →
      isCorrectPC (WCap pc_p pc_g pc_b pc_e pc_a) →
-
+     (pc_a + imm)%a = Some pc_a' →
      {{{ ▷ PC ↦ᵣ WCap pc_p pc_g pc_b pc_e pc_a
-         ∗ ▷ pc_a ↦ₐ w }}}
-       Instr Executable @ E
-       {{{ RET NextIV;
-           PC ↦ᵣ updatePcPerm (WCap pc_p pc_g pc_b pc_e pc_a)
-           ∗ pc_a ↦ₐ w }}}.
-  Proof.
-    iIntros (Hinstr Hvpc ϕ) "(>HPC & >Hpc_a) Hφ".
-    iApply wp_lift_atomic_base_step_no_fork; auto.
-    iIntros (σ1 ns l1 l2 nt) "[ [Hr0 Hsr] Hm ] /=". destruct σ1 as [ [r0 sr] m]; cbn.
-    iDestruct (@gen_heap_valid with "Hm Hpc_a") as %?; auto.
-    iDestruct (@gen_heap_valid with "Hr0 HPC") as %Hr_PC.
-    iModIntro. iSplitR. by iPureIntro; apply normal_always_base_reducible.
-    iNext. iIntros (e2 σ2 efs Hpstep).
-    apply prim_step_exec_inv in Hpstep as (-> & -> & (c & -> & Hstep)).
-    iIntros "_".
-    iSplitR; auto. eapply step_exec_inv in Hstep; eauto.
-    unfold exec, exec_opt in Hstep. rewrite Hr_PC /= in Hstep. simplify_pair_eq.
+         ∗ ▷ pc_a ↦ₐ w
+         ∗ ▷ rimm ↦ᵣ WInt imm
+     }}}
+       Instr Executable @ Ep
+     {{{ RET NextIV;
+         PC ↦ᵣ WCap pc_p pc_g pc_b pc_e pc_a'
+         ∗ pc_a ↦ₐ w
+         ∗ rimm ↦ᵣ WInt imm
+     }}}.
+   Proof.
+     iIntros (Hinstr Hvpc Hpca' ϕ) "(>HPC & >Hpc_a & >Hrimm) Hφ".
+     iDestruct (map_of_regs_2 with "HPC Hrimm") as "[Hmap %]".
+     iApply (wp_Jmp with "[$Hmap Hpc_a]"); eauto; simplify_map_eq; eauto.
+     { set_solver+. }
+     iNext. iIntros (regs' retv) "(%Hspec & Hpc_a & Hmap)".
 
-    iMod (@gen_heap_update with "Hr0 HPC") as "[Hr0 HPC]". iFrame.
-    iApply "Hφ". by iFrame.
-  Qed.
+     destruct Hspec as [| * Hfail].
+     { (* Success *)
+       iApply "Hφ". iFrame.
+       incrementPC_inv as (?&?&?&?&?&?&?&?&?); simplify_map_eq.
+       rewrite insert_insert //.
+       iDestruct (regs_of_map_2 with "Hmap") as "(?&?)"; eauto; iFrame. }
+     { (* Failure (contradiction) *)
+       destruct Hfail; simplify_map_eq; eauto; try congruence.
+       incrementPC_inv as (?&?&?&?&?&?&?&?&?); simplify_map_eq; eauto ; congruence.
+     }
+   Qed.
+
 
 End cap_lang_rules.
