theories/ftlr/Jalr.v
@@ -1,0 +1,134 @@
+From cap_machine Require Export logrel.
+From iris.proofmode Require Import proofmode.
+From iris.program_logic Require Import weakestpre adequacy lifting.
+From stdpp Require Import base.
+From cap_machine.ftlr Require Import ftlr_base interp_weakening.
+From cap_machine.rules Require Import rules_base rules_Jalr.
+From cap_machine.proofmode Require Import map_simpl register_tactics.
+
+Section fundamental.
+  Context
+    {Σ : gFunctors}
+      {ceriseg: ceriseG Σ} {sealsg: sealStoreG Σ}
+      {stsg : STSG Addr region_type Σ} {heapg : heapGS Σ}
+      {nainv: logrel_na_invs Σ}
+      {MP: MachineParameters}.
+
+  Notation STS := (leibnizO (STS_states * STS_rels)).
+  Notation STS_STD := (leibnizO (STS_std_states Addr region_type)).
+  Notation WORLD := (prodO STS_STD STS).
+  Implicit Types W : WORLD.
+
+  Notation D := (WORLD -n> (leibnizO Word) -n> iPropO Σ).
+  Notation R := (WORLD -n> (leibnizO Reg) -n> iPropO Σ).
+  Implicit Types w : (leibnizO Word).
+  Implicit Types interp : (D).
+
+
+  Lemma jalr_case (W : WORLD) (regs : leibnizO Reg)
+    (p p': Perm) (g : Locality) (b e a : Addr)
+    (w : Word) (ρ : region_type) (rdst : RegName) (P:D):
+    ftlr_instr W regs p p' g b e a w (Jalr rdst) ρ P.
+  Proof.
+    intros Hp Hsome HcorrectPC Hbae Hfp HO Hpers Hpwl Hregion Hnotrevoked Hnotfrozen Hi.
+    iIntros "#IH #Hinv_interp #Hreg #Hinva #Hrcond #Hwcond #Hmono #HmonoV Hw Hsts Hown".
+    iIntros "Hr Hstate Ha HPC Hmap".
+    iInsert "Hmap" PC.
+    iApply (wp_Jalr with "[$Ha $Hmap]"); eauto.
+    { simplify_map_eq; auto. }
+    { rewrite /subseteq /map_subseteq. intros rr _.
+      apply elem_of_dom. apply lookup_insert_is_Some'; eauto. }
+
+    iIntros "!>" (regs' retv). iDestruct 1 as (HSpec) "[Ha Hmap]".
+    destruct HSpec as [ regs' pc_a' wdst Hrdst Hpca' ->| Hpca' ]; cycle 1.
+    {
+      iApply wp_pure_step_later; auto. iNext; iIntros "_".
+      iApply wp_value; auto. iIntros; discriminate.
+    }
+
+    rewrite (insert_commute _ cra PC) // insert_insert.
+    iApply wp_pure_step_later; auto.
+
+    iAssert (interp W (WCap (seal_perm_sentry p) g b e pc_a')) as "Hinterp_ret".
+    { pose proof (isCorrectPC_nonSentry p _ _ _ _ HcorrectPC ) as HpnotSentry.
+      iApply (interp_weakening with "IH Hinv_interp");eauto;try solve_addr.
+      - rewrite /seal_perm_sentry; destruct p ; cbn in HpnotSentry; try congruence.
+        repeat (apply andb_True;split; try reflexivity).
+        destruct Hp as [Hexec _].
+        destruct rx; cbn in Hexec ; try congruence;done.
+      - reflexivity.
+    }
+
+    destruct (updatePcPerm wdst) eqn:Hwdst ; [ | destruct sb | ]; cycle 1.
+    { destruct (executeAllowed p0) eqn:Hpft; cycle 1.
+      { iNext; iIntros "_".
+        iApply (wp_bind (fill [SeqCtx])).
+        iExtract "Hmap" PC as "HPC".
+        iApply (wp_notCorrectPC with "HPC"); [eapply not_isCorrectPC_perm; naive_solver|].
+        iNext; iIntros "HPC /=".
+        iApply wp_pure_step_later; auto; iNext; iIntros "_".
+        iApply wp_value; iIntros; discriminate.
+      }
+
+
+      destruct_word wdst; cbn in Hwdst; try discriminate.
+      destruct c; inv Hwdst.
+      { iNext ; iIntros "_".
+        iDestruct (region_close with "[$Hstate $Hr $Ha $HmonoV Hw]") as "Hr"; eauto.
+        { destruct ρ;auto;[|ospecialize (Hnotfrozen _)];contradiction. }
+        iApply ("IH" $! _ (<[cra:=WCap (seal_perm_sentry p) g b e pc_a']> regs) with "[%] [] [Hmap] [$Hr] [$Hsts] [$Hown]") ; eauto.
+        - intros; cbn.
+          rewrite lookup_insert_is_Some.
+          destruct (decide (cra = x)); auto; right; split; auto.
+        - iIntros (ri wi Hri Hregs_ri).
+          destruct (decide (ri = cra)); simplify_map_eq; cycle 1.
+          * iApply ("Hreg" $! ri) ; auto.
+          * iFrame "Hinterp_ret".
+        - destruct (decide (rdst = PC)) as [HrdstPC|HrdstPC].
+          + simplify_map_eq; auto.
+          + simplify_map_eq.
+            iDestruct ("Hreg" $! rdst _ HrdstPC Hrdst) as "Hrdst"; eauto.
+      }
+      { assert (rdst <> PC) as HPCnrdst.
+        { intro; subst rdst; simplify_map_eq.
+          destruct Hp as [Hexec _]
+          ; eapply executeAllowed_nonSentry in Hexec
+          ; eauto ; cbn in Hexec
+          ; naive_solver.
+        }
+        simplify_map_eq.
+        iDestruct ("Hreg" $! rdst _ HPCnrdst Hrdst) as "Hwdst".
+        iEval (rewrite fixpoint_interp1_eq) in "Hwdst".
+        simpl; rewrite /enter_cond.
+        iDestruct "Hwdst" as "#Hinterp_dst".
+        iAssert (future_world g0 W W) as "Hfuture".
+        { iApply futureworld_refl. }
+
+        iSpecialize ("Hinterp_dst" with "Hfuture").
+        iDestruct "Hinterp_dst" as "[Hinterp_dst _]".
+        iDestruct (region_close with "[$Hstate $Hr Hw $Ha $HmonoV]") as "Hr"; eauto.
+        { destruct ρ;auto;[|ospecialize (Hnotfrozen _)];contradiction. }
+        iDestruct ("Hinterp_dst" with "[$Hmap $Hr $Hsts $Hown]") as "HA"; eauto.
+        iNext.
+        cbn; iSplit.
+        - iIntros (ri); cbn; iPureIntro.
+          rewrite lookup_insert_is_Some.
+          destruct (decide (cra = ri)); auto; right; split; auto.
+        - iIntros (ri wi Hri Hregs_ri).
+          destruct (decide (ri = cra)); simplify_map_eq; cycle 1.
+          * iApply ("Hreg" $! ri) ; auto.
+          * iFrame "Hinterp_ret".
+      }
+    }
+
+    (* Non-capability cases *)
+    all: iExtract "Hmap" PC as "HPC".
+    all: iNext; iIntros "_".
+    all: iApply (wp_bind (fill [SeqCtx])).
+    all: iApply (wp_notCorrectPC with "HPC"); [intro Hcontra ; inv Hcontra|].
+    all: iNext; iIntros "HPC /=".
+    all: iApply wp_pure_step_later; auto; iNext; iIntros "_".
+    all: iApply wp_value; iIntros; discriminate.
+  Qed.
+
+End fundamental.
