theories/ftlr/Jmp.v
@@ -1,9 +1,9 @@
+From cap_machine Require Export logrel.
 From iris.proofmode Require Import proofmode.
 From iris.program_logic Require Import weakestpre adequacy lifting.
 From stdpp Require Import base.
-From cap_machine Require Export logrel.
-From cap_machine.ftlr Require Import ftlr_base.
-From cap_machine.rules Require Import rules_Jmp.
+From cap_machine.ftlr Require Import ftlr_base interp_weakening.
+From cap_machine.rules Require Import rules_base rules_Jmp.
 From cap_machine.proofmode Require Import map_simpl register_tactics.
 
 Section fundamental.
@@ -24,82 +24,35 @@ Section fundamental.
   Implicit Types w : (leibnizO Word).
   Implicit Types interp : (D).
 
-
   Lemma jmp_case (W : WORLD) (regs : leibnizO Reg)
     (p p': Perm) (g : Locality) (b e a : Addr)
-    (w : Word) (ρ : region_type) (rsrc : RegName) (P:D):
-    ftlr_instr W regs p p' g b e a w (Jmp rsrc) ρ P.
+    (w : Word) (ρ : region_type) (rimm : Z + RegName) (P:D):
+    ftlr_instr W regs p p' g b e a w (Jmp rimm) ρ P.
   Proof.
     intros Hp Hsome HcorrectPC Hbae Hfp HO Hpers Hpwl Hregion Hnotrevoked Hnotfrozen Hi.
     iIntros "#IH #Hinv_interp #Hreg #Hinva #Hrcond #Hwcond #Hmono #HmonoV Hw Hsts Hown".
     iIntros "Hr Hstate Ha HPC Hmap".
-    destruct (decide (rsrc = PC)) as [HrPC|HrPC].
-    - subst rsrc.
-      iApply (wp_jmp_successPC with "[HPC Ha]"); eauto; first iFrame.
-      iNext. iIntros "[HPC Ha] /=".
-      iApply wp_pure_step_later; auto.
-      (* reconstruct regions *)
-      iNext; iIntros "_".
-      iInsert "Hmap" PC.
-      (* close region *)
-      iDestruct (region_close with "[$Hstate $Hr Hw $Ha $HmonoV]") as "Hr"; eauto.
-      { destruct ρ;auto;[|specialize (Hnotfrozen g0)];contradiction. }
-      (* apply IH *)
-      iApply ("IH" $! _ _ _ g _ _ a with "[] [] [Hmap] [$Hr] [$Hsts] [$Hown]"); eauto.
-      { iPureIntro; apply Hsome. }
-      destruct p
-      ; iFrame
-      ; apply isCorrectPC_nonSentry in HcorrectPC; by cbn in HcorrectPC.
-    - specialize Hsome with rsrc as Hrsrc; destruct Hrsrc as [wsrc Hsomesrc].
-      iExtract "Hmap" rsrc as "Hrsrc".
-      iApply (wp_jmp_success with "[$HPC $Ha $Hrsrc]"); eauto.
-      iNext. iIntros "[HPC [Ha Hrsrc]] /=".
-      iApply wp_pure_step_later; auto.
-      (* reconstruct regions *)
-      iInsert "Hmap" rsrc;
-      rewrite -delete_insert_ne; auto.
-      destruct (updatePcPerm wsrc) eqn:Heq ; [ | destruct sb | ]; cycle 1.
-      { destruct (executeAllowed p0) eqn:Hpft; cycle 1.
-        { iNext; iIntros "_".
-          iApply (wp_bind (fill [SeqCtx])).
-          iApply (wp_notCorrectPC with "HPC"); [eapply not_isCorrectPC_perm; naive_solver|].
-          iNext; iIntros "HPC /=".
-          iApply wp_pure_step_later; auto; iNext; iIntros "_".
-          iApply wp_value; iIntros; discriminate.
-        }
-        iInsert "Hmap" PC.
-        rewrite (insert_id regs rsrc); auto.
-        iDestruct ("Hreg" $! rsrc _ HrPC Hsomesrc) as "Hwsrc".
-        destruct wsrc; simpl in Heq; try congruence.
-        destruct sb as [p1 g1 b1 e1 a1|?]; try congruence.
-        destruct p1 as [rx pw dl dro | rx pw dl dro] ; cycle 1; simplify_eq.
-        + (* case p1 = E *)
-          iEval (rewrite fixpoint_interp1_eq) in "Hwsrc".
-          simpl; rewrite /enter_cond.
-          iDestruct "Hwsrc" as "#H".
-          iAssert (future_world g0 W W) as "Hfuture".
-          { iApply futureworld_refl. }
-          iSpecialize ("H" with "Hfuture").
-          iDestruct "H" as "[H _]".
-          iDestruct (region_close with "[$Hstate $Hr Hw $Ha $HmonoV]") as "Hr"; eauto.
-          { destruct ρ;auto;[|ospecialize (Hnotfrozen _)];contradiction. }
-          iDestruct ("H" with "[$Hmap $Hr $Hsts $Hown]") as "HA"; eauto.
-          iFrame "#%".
-        + (* case p1 ≠ E *)
-          iEval (rewrite fixpoint_interp1_eq) in "Hinv_interp".
-          iNext; iIntros "_".
-          iDestruct (region_close with "[$Hstate $Hr Hw $Ha $HmonoV]") as "Hr"; eauto.
-          { destruct ρ;auto;[|ospecialize (Hnotfrozen _)];contradiction. }
-          iApply ("IH" with "[] [] [$Hmap] [$Hr] [$Hsts] [$Hown]"); eauto.
-      }
+    iInsert "Hmap" PC.
+    iApply (wp_Jmp with "[$Ha $Hmap]"); eauto.
+    { simplify_map_eq; auto. }
+    { rewrite /subseteq /map_subseteq. intros rr _.
+      apply elem_of_dom. apply lookup_insert_is_Some'; eauto. }
 
-      (* Non-capability cases *)
-      all: iNext; iIntros "_".
-      all: iApply (wp_bind (fill [SeqCtx])).
-      all: iApply (wp_notCorrectPC with "HPC"); [intro Hcontra ; inv Hcontra|].
-      all: iNext; iIntros "HPC /=".
-      all: iApply wp_pure_step_later; auto; iNext; iIntros "_".
-      all: iApply wp_value; iIntros; discriminate.
+    iIntros "!>" (regs' retv). iDestruct 1 as (HSpec) "[Ha Hmap]".
+    destruct HSpec as [ regs' imm Himm Hincr| ]; cycle 1.
+    {
+      iApply wp_pure_step_later; auto. iNext; iIntros "_".
+      iApply wp_value; auto. iIntros; discriminate.
+    }
+
+    incrementPC_inv as (p0&g0&b0&e0&a0&a0'&?&Ha0'&?); simplify_map_eq.
+    rewrite insert_insert.
+    iApply wp_pure_step_later; auto. iNext; iIntros "_".
+    iDestruct (region_close with "[$Hstate $Hr $Ha $HmonoV Hw]") as "Hr"; eauto.
+    { destruct ρ;auto;[|ospecialize (Hnotfrozen _)];contradiction. }
+    iApply ("IH" $! _ regs with "[%] [] [Hmap] [$Hr] [$Hsts] [$Hown]") ; eauto.
+    iApply (interp_weakening with "IH Hinv_interp"); eauto; try solve_addr; try reflexivity.
+    by eapply isCorrectPC_nonSentry.
   Qed.
 
 End fundamental.
