theories/rules.v
@@ -2,8 +2,8 @@
    with one file for each instruction, which we import below. *)
 From cap_machine.rules Require Export
      rules_Get rules_Load rules_Store rules_BinOp
-     rules_Lea rules_Mov rules_Restrict
-     rules_Jmp rules_Jnz rules_Subseg
+     rules_Lea rules_Mov rules_Restrict rules_Subseg
+     rules_Jmp rules_Jnz rules_Jalr
      rules_Seal rules_UnSeal
      rules_ReadSR rules_WriteSR.
 
